progress on correctness proof

theories/compiler/mem2reg.v
@@ -12,6 +12,7 @@ Require Import refframe.imp.
 Require Export refframe.compiler.monad.
 Require Export refframe.compiler.linear_imp.
 Require Export refframe.compiler.linearize.
+Require Import refframe.imp_heap_bij_own.
 
 
 Module ci2a_mem2reg.
@@ -23,6 +24,16 @@ Definition M := compiler_monad unit (fn_compiler_monoid lexpr) error.
 
 Definition is_var (e: var_val) (x: string) :=
   if e is (VVar y) then bool_decide (x = y) else false.
+
+Lemma is_var_dec v x: is_var v x = bool_decide (v = VVar x).
+Proof.
+  rewrite /is_var. destruct v;
+    rewrite !bool_decide_decide; destruct decide.
+  - subst. destruct decide; naive_solver.
+  - destruct decide; naive_solver.
+  - naive_solver.
+  - naive_solver.
+Qed.
 
 
 Definition lexpr_op_pass (x: string) (e: lexpr_op) : M lexpr_op :=
@@ -42,8 +53,9 @@ Definition lexpr_op_pass (x: string) (e: lexpr_op) : M lexpr_op :=
       mret $ LVarVal v2
     else mret $ LStore v1 v2
   | LCall f args =>
-    vs ← cmap args 0 (λ _ v, if is_var v x then cerror UsedAsLoc else mret $ v);
-    mret $ (LCall f vs)
+    cassert UsedAsLoc (Forall (λ v, is_var v x = false) args);;
+    (* vs ← cmap args 0 (λ _ v, if is_var v x then  else mret $ v); *)
+    mret (LCall f args)
   | LUbE => mret $ LUbE
   end.
 
@@ -51,7 +63,7 @@ Fixpoint pass (x: string) (e : lexpr) : M lexpr :=
   match e with
   | LLetE v e1 e2 =>
     if bool_decide (v = x) then
-      '(e1', _) ← cscope (lexpr_op_pass x e1);
+      e1' ← lexpr_op_pass x e1;
       mret $ LLetE v e1' e2
     else
       '(e1', upd) ← cscope (lexpr_op_pass x e1);
@@ -71,14 +83,23 @@ Fixpoint pass (x: string) (e : lexpr) : M lexpr :=
   end.
 
 
-Definition pass_fn (f : lfndef) : lfndef :=
-  let (e, vars) := foldr (λ '(x, n) '(r, vars),
-    let res := crun () (pass x r) in
+Definition pass_single_var (x: string) (e: lexpr) (vars: list (string * Z)) :=
+  let res := crun () (pass x e) in
+  match list_find (λ '(y, n), bool_decide (y = x)) vars with
+  | None => (e, vars)
+  | Some (i, _) =>
     match res.(c_result) with
-    | CSuccess r' => (LLetE x (LVarVal (VVal (StaticValNum 0))) r', vars)
-    | CError _ => (r, (x, n)::vars)
+    | CSuccess e' => (LLetE x (LVarVal (VVal (StaticValNum 0))) e', delete i vars)
+    | CError _ => (e, vars)
     end
-  ) (f.(lfd_body), []) f.(lfd_vars) in
+  end.
+
+Definition pass_body (e: lexpr) (vars: list (string * Z)) :=
+  foldr (λ '(x, n) '(r, vars), pass_single_var x r vars) (e, vars) vars.
+
+
+Definition pass_fn (f : lfndef) : lfndef :=
+  let (e, vars) := pass_body f.(lfd_body) f.(lfd_vars) in
   {|
      lfd_args := f.(lfd_args);
      lfd_vars := vars;
@@ -127,5 +148,259 @@ Definition test_fn_3 : fndef := {|
 
 Compute test_opt_fn test_fn_3.
 
+(*
+Lemma pass_lookup_singleton (f g: string) fn fn':
+  (lfndef_to_fndef <$> <[f:=fn]> ∅: gmap string fndef) !! g = Some fn' →
+  fn' = lfndef_to_fndef fn ∧ f = g.
+Proof.
+  rewrite !lookup_fmap.
+  intros [x [Hlook ->]]%fmap_Some_1.
+  eapply lookup_insert_Some in Hlook as [[-> <-]|[? ?]]; last set_solver.
+  done.
+Qed. *)
+
+
+Lemma subst_map_var_val_identical x v vss vsi:
+  (∀ y, y ≠ x → vss !! y = vsi !! y) →
+  v ≠ VVar x →
+  subst_map vss (var_val_to_expr v) = subst_map vsi (var_val_to_expr v).
+Proof.
+  destruct v as [y|]; last done.
+  intros Hlook Hneq.
+  assert (y ≠ x) as Heq%Hlook by naive_solver.
+  rewrite /= Heq //.
+Qed.
+
+
+Lemma pass_lexpr_op_correct ei' Ki ei Ks es es' x (l: loc) n hi hs fns1 fns2 vsi vss w rf upd
+  `{Hfill1: !ImpExprFill es Ks (subst_map vss (lexpr_op_to_expr es'))}
+  `{Hfill2: !ImpExprFill ei Ki (subst_map vsi (lexpr_op_to_expr ei'))}:
+    imp_heap_bij_proof_call n fns1 fns2 →
+    crun () (lexpr_op_pass x es') = CResult () upd (CSuccess ei') →
+    (∀ y, y ≠ x → vsi !! y = vss !! y) →
+    vss !! x = Some (ValLoc l) →
+    vsi !! x = Some w →
+    (* This should become local ownership eventually *)
+    hs.(h_heap) !! l = Some w →
+    Imp ei hi fns1
+      ⪯{imp_module, imp_heap_bij imp_module, n, true}
+    (SMProg, Imp es hs fns2, (PPInside, (), rf)).
+Proof.
+  intros Hbij Hrun Hlook Hxs Hxi Hl; destruct es' as [v|v1 op v2|v|v1 v2|y vs|]; simpl in Hrun.
+  - rewrite is_var_dec bool_decide_decide in Hrun.
+    destruct decide; first by eapply cerror_success in Hrun.
+    eapply cret_success in Hrun as (_ & ? & ?); subst.
+    simpl in Hfill1, Hfill2.
+    admit.
+  - rewrite is_var_dec bool_decide_decide in Hrun.
+    destruct decide; first by eapply cerror_success in Hrun.
+    rewrite is_var_dec bool_decide_decide in Hrun.
+    destruct decide; first by eapply cerror_success in Hrun.
+    eapply cret_success in Hrun as (_ & ? & ?); subst.
+    simpl in Hfill1, Hfill2.
+    admit.
+  - rewrite is_var_dec bool_decide_decide in Hrun.
+    destruct decide; eapply cret_success in Hrun as (_ & ? & ?); subst.
+    + simpl in Hfill1, Hfill2.
+      rewrite Hxs in Hfill1; rewrite Hxi in Hfill2.
+      tstep_s. intros ??; injection 1 as <-; intros ?.
+      simplify_eq.
+      admit. (* there the continuation should apply *)
+    + simpl in Hfill1, Hfill2.
+      (* We should be able to proceed with the load here.
+         Still need to fix the substitution stuff. *)
+      tstep_both. admit.
+  - rewrite !is_var_dec !bool_decide_decide in Hrun.
+    destruct decide; first by eapply cerror_success in Hrun.
+    destruct decide.
+    + admit.
+    + eapply cret_success in Hrun as (_ & ? & ?); subst.
+      simpl in Hfill1, Hfill2.
+      (* We should be able to proceed with the load here.
+         Still need to fix the substitution stuff. *)
+      tstep_both. admit.
+  - eapply cbind_success in Hrun as ([] & g & vs' & ? & Hrun1 & Hrun2 & ->).
+    eapply cret_success in Hrun2 as (_ & ? & ?); subst.
+    eapply cassert_success in Hrun1 as (_ & ? & ? & ?); subst.
+    simpl in Hfill1, Hfill2.
+    eapply Hbij; eauto.
+    (* we need the function call case here *)
+    all: admit.
+  - eapply cret_success in Hrun as (_ & ? & ?); subst.
+    simpl in Hfill1, Hfill2.
+    tstep_s. done.
+  Admitted.
+
+Lemma pass_correct ei' Ki ei Ks es es' x n h h' fns1 fns2 vsi vss rf r_p
+  `{Hfill1: !ImpExprFill es Ks (subst_map vss (lexpr_to_expr es'))}
+  `{Hfill2: !ImpExprFill ei Ki (subst_map vsi (lexpr_to_expr ei'))}:
+    imp_heap_bij_proof_call n fns1 fns2 →
+    crun () (pass x es') = CResult () r_p (CSuccess ei') →
+    Imp ei h fns1
+      ⪯{imp_module, imp_heap_bij imp_module, n, true}
+    (SMProg, Imp es h' fns2, (PPInside, (), rf)).
+Proof.
+  revert ei' Ki ei Ks es x n h h' fns1 fns2 vsi vss rf r_p Hfill1 Hfill2.
+  induction es' as [y op es' IH| op es1' IH1 es2' IH2 | op];
+    intros ei' Ki ei Ks es x n h h' fns1 fns2 vsi vss rf r_p Hfill1 Hfill2;
+    intros Hcall Hrun; simpl in Hrun.
+  - rewrite bool_decide_decide in Hrun.
+    destruct decide.
+    + subst. eapply cbind_success in Hrun as ([] & a2 & r2 & a3' & Hrun1 & Hrun2 & ->).
+      eapply cret_success in Hrun2 as (_ & -> & ->).
+      simpl in Hfill1, Hfill2.
+      admit.
+    + eapply cbind_success in Hrun as ([] & a2 & [e1' upd] & a3' & Hrun1 & Hrun2 & ->).
+      eapply cbind_success in Hrun2 as ([] & a2' & r2 & ? & Hrun2 & Hrun3 & ->).
+      eapply cret_success in Hrun3 as (_ & -> & ->).
+      admit.
+  - admit.
+  - admit.
+Admitted.
+
+(*
+Lemma pass_body_correct ei' Ki ei Ks es es' n h h' fns1 fns2 vin vout vsi vss  rf
+      `{Hfill1: !ImpExprFill es Ks (subst_map vss (lexpr_to_expr es'))}
+      `{Hfill2: !ImpExprFill ei Ki (subst_map vsi (lexpr_to_expr ei'))}:
+  imp_heap_bij_proof_call n fns1 fns2 →
+  (pass_body es' vin) = (ei', vout) →
+  (* (∀ h' v' vsi',
+    (s ≤ s')%N →
+    lookup_var_val vsi' v = Some v' →
+    vsi ⊆ vsi' →
+    (∀ v, is_Some (vsi' !! v) → is_Some (vsi !! v) ∨
+                                v ∈ assigned_vars (static_expr_to_expr es') ∨
+                                ∃ n, v = tmp_var n ∧ (n < s')%N) →
+    Imp (expr_fill Ki $ subst_map vsi' (lexpr_to_expr ei')) h' fns1
+       ⪯{imp_module, imp_module, n, false}
+    Imp (expr_fill Ks (Val v')) h' fns2) → *)
+  Imp ei h fns1
+      ⪯{imp_module, imp_heap_bij imp_module, n, true}
+  (SMProg, Imp es h' fns2, (PPInside, (), rf)).
+Proof. Admitted. *)
+  (* revert ei' Ki ei Ks es es' n h h' fns1 fns2 vout vsi vss vs1 vs2 r rf Hfill1 Hfill2.
+  induction vin as [|[s k] vin IH]; simpl;
+    intros ei' Ki ei Ks es es' n h h' fns1 fns2 vout vsi vss vs1 vs2 r rf Hfill1 Hfill2;
+    intros Hcall Hpass Hsat.
+  - injection Hpass as ? <-.
+    subst ei'. admit.
+    (* FIXME: we need some kind of reflexivity here, with *)
+  - destruct (pass_body es' vin) as [es'' vars''] eqn: Hbody.
+    destruct (crun () (pass s es'')) as [r_s r_p [res|err]] eqn: Hpass_var;
+      simpl in Hpass.
+    + injection Hpass as ? ?. subst vout ei'. admit.
+      (* FIXME: to proceed here, I think we need transitivity.
+        We need to compose the refinement of the recursively
+        optimized function with the one optimization pass we add now. *)
+
+    + injection Hpass as ??. subst ei' vout.
+      eapply IH; eauto.
+Admitted. *)
+
+
+Lemma pass_single_var_correct f x args exprs varss expri varsi :
+  pass_single_var x exprs varss = (expri, varsi) →
+  trefines
+  (MS (imp_heap_bij imp_module)
+     (initial_imp_heap_bij_state imp_module
+        (initial_imp_state
+           (lfndef_to_fndef <$>
+            <[f:={| lfd_args := args; lfd_vars := varsi; lfd_body := expri |}]> ∅))))
+  (MS (imp_heap_bij imp_module)
+     (initial_imp_heap_bij_state imp_module
+        (initial_imp_state
+           (lfndef_to_fndef <$>
+            <[f:={| lfd_args := args; lfd_vars := varss; lfd_body := exprs |}]> ∅)))).
+Proof.
+  rewrite /pass_single_var.
+  destruct list_find as [[i [y n]]|] eqn: Hfind;
+    first destruct (crun () (pass x exprs)) as [[] ? [res|]]; simpl;
+    last first.
+  - injection 1 as ??; subst. reflexivity.
+  - injection 1 as ??; subst. reflexivity.
+  - injection 1 as ??; subst.
+Admitted.
+
+
+Lemma pass_body_correct f args varss exprs expri varsi:
+  pass_body exprs varss = (expri, varsi) →
+  trefines
+    (MS (imp_heap_bij imp_module)
+       (initial_imp_heap_bij_state imp_module
+          (initial_imp_state
+             (lfndef_to_fndef <$>
+              <[f:={| lfd_args := args; lfd_vars := varsi; lfd_body := expri |}]> ∅))))
+    (MS (imp_heap_bij imp_module)
+       (initial_imp_heap_bij_state imp_module
+          (initial_imp_lstate
+             (<[f:={| lfd_args := args; lfd_vars := varss; lfd_body := exprs |}]> ∅)))).
+Proof.
+  rewrite /pass_body. generalize varss at 2 as L.
+  induction L as [|[x n] L IHL] in varss, varsi, exprs, expri |-*; simpl.
+  - injection 1 as ??. subst; reflexivity.
+  - destruct foldr as [expri' varsi'] eqn: Hbody.
+    intros Hsingle.
+    eapply IHL in Hbody as IH.
+    etrans; last eapply IH. eapply pass_single_var_correct, Hsingle.
+Qed.
+
+Lemma pass_fn_correct f fn :
+  trefines (MS imp_module (initial_imp_lstate (<[f := pass_fn fn]> ∅)))
+           (MS (imp_heap_bij imp_module) (initial_imp_heap_bij_state imp_module
+                                            (initial_imp_lstate (<[f := fn]> ∅)))).
+Proof.
+  etrans; first eapply imp_heap_bij_imp_refl.
+  rewrite /pass_fn. destruct pass_body as [expri varsi] eqn: Hpass.
+  revert Hpass. destruct fn as [args varss exprs]; simpl.
+  by eapply pass_body_correct.
+Qed.
+
+(*
+Lemma pass_fn_correct f fn :
+  trefines (MS imp_module (initial_imp_lstate (<[f := pass_fn fn]> ∅)))
+           (MS (imp_heap_bij imp_module) (initial_imp_heap_bij_state imp_module
+                                            (initial_imp_lstate (<[f := fn]> ∅)))).
+Proof.
+  apply: imp_heap_bij_proof. { set_solver. }
+  - move => ??. intros [-> ->]%pass_lookup_singleton.
+    eexists. split; simpl.
+    { rewrite lookup_fmap. eapply fmap_Some_2, lookup_insert.  }
+    { destruct fn; unfold pass_fn, pass_body; simpl. by destruct foldr. }
+  - intros n K1 K2 g fn1 fn2 vs1 vs2 h1 h2 r rf.
+    intros [-> ->]%pass_lookup_singleton.
+    intros [-> _]%pass_lookup_singleton.
+    intros Hlen1 Hlen2 Hsat Hcalls Hcont.
+    destruct fn; simpl. unfold pass_fn; simpl.
+    destruct (pass_body) as [e' vars'] eqn: Hpass; simpl.
+    tstep_both. intros ls h' Halloc. tstep_s.
+    edestruct (heap_alloc_list_fresh lfd_vars.*2 ∅ h2) as [h Heap].
+    eexists _, _. split; first done.
+    intros Hall. tend. split.
+    { eapply List.Forall_forall.
+      intros x [s [-> Hel]]%elem_of_list_In%elem_of_list_fmap_2.
+      eapply pass_body_vars in Hel; last done.
+      eapply List.Forall_forall; first done.
+      eapply elem_of_list_In, elem_of_list_fmap_1, Hel. }
+    rewrite !fmap_insert fmap_empty.
+    rewrite !subst_l_subst_map; first last.
+    { eapply heap_alloc_list_length in Halloc.
+      revert Halloc. rewrite !fmap_length //.  }
+    { revert Hlen1. rewrite /pass_fn //=.
+      rewrite Hpass //. }
+    { rewrite !fmap_length. clear. unfold fmap.
+      generalize (∅: (gset prov)). generalize h2.
+      induction lfd_vars as [|[]? IH]; simpl; first done.
+      intros ??. by erewrite IH. }
+    { revert Hlen1. rewrite /pass_fn //=. }
+    rewrite -!subst_map_subst_map.
+    rewrite -!list_to_map_app.
+    eapply pass_body_correct.
+    + eapply imp_expr_fill_expr_fill, imp_expr_fill_FreeA, imp_expr_fill_end.
+    + eapply imp_expr_fill_expr_fill, imp_expr_fill_FreeA, imp_expr_fill_end.
+    + revert Hcalls. rewrite !fmap_insert fmap_empty /pass_fn //=.
+      rewrite Hpass //.
+    + done.
+    + done.
+  Qed. *)
 
 End ci2a_mem2reg.
